isabelle/CompileAll.thy
@@ -5,7 +5,7 @@ imports
   Chapter09_3_Evaluation
   Chapter10_3_Evaluation
   Chapter11_3_Evaluation
-  Chapter12_3_Evaluation
+  Chapter12_4_Evaluation
   Chapter15_3_Evaluation
   Chapter16_5_Abbreviation
   Chapter17
